James C - slight cleanup, set into total correctness

AssemblyLanguage.thy
@@ -2,18 +2,16 @@ theory AssemblyLanguage
 imports FiniteMap BasicComputation
 begin
 
-typedecl symbol
-
 datatype assembly =
   AAssm int
 | CAssm "register set" computation
 | JAssm "comparison set" symbol
 
-type_synonym program = "symbol \<leadsto> assembly list"
+type_synonym assembly_program = "symbol \<leadsto> assembly list"
 
 type_synonym assembly_state = "memory \<times> int option \<times> int \<times> assembly list" (* \<mu>, a, d, pc *)
 
-fun eval_assembly :: "program \<Rightarrow> assembly_state \<Rightarrow> assembly_state option" where
+fun eval_assembly :: "assembly_program \<Rightarrow> assembly_state \<Rightarrow> assembly_state option" where
   "eval_assembly \<Pi> (\<mu>, a, d, []) = None"
 | "eval_assembly \<Pi> (\<mu>, a, d, AAssm x # \<pi>) = Some (\<mu>, Some x, d, \<pi>)"
 | "eval_assembly \<Pi> (\<mu>, Some a, d, CAssm dst cmp # \<pi>) = (
