MachineLanguage.thy
@@ -6,6 +6,8 @@ datatype machine_instruction =
   AInstr int
 | CInstr "register set" computation "comparison set"
 
+type_synonym machine_program = "machine_instruction list"
+
 type_synonym machine_state = "memory \<times> int \<times> int \<times> nat" (* \<mu>, a, d, pc *)
 
 fun eval_instruction :: "machine_instruction \<Rightarrow> machine_state \<Rightarrow> machine_state" where
@@ -17,7 +19,7 @@ fun eval_instruction :: "machine_instruction \<Rightarrow> machine_state \<Right
         if D \<in> dst then n else d, 
         if should_jump n jmp then nat a else Suc pc))"
 
-fun eval_machine :: "machine_instruction list \<Rightarrow> machine_state \<Rightarrow> machine_state option" where
+fun eval_machine :: "machine_program \<Rightarrow> machine_state \<Rightarrow> machine_state option" where
   "eval_machine \<Pi> (\<mu>, a, d, pc) = (
     if pc < length \<Pi> 
     then Some (eval_instruction (\<Pi> ! pc) (\<mu>, a, d, pc)) 
