StackToAssembly.thy
@@ -1,10 +1,116 @@
 theory StackToAssembly
-imports StackMachine
+imports StackLanguage AssemblyLanguage Iterate
 begin
 
+primrec instruction_conv :: "stack_instruction \<Rightarrow> assembly list" where
+  "instruction_conv Add = [AAssm 0, CAssm {A} (Reg M), CAssm {D} (Reg M), AAssm 0, CAssm {A, M} (Decr M), CAssm {M} DPlusM]"
+| "instruction_conv Sub = [AAssm 0, CAssm {A} (Reg M), CAssm {D} (Reg M), AAssm 0, CAssm {A, M} (Decr M), CAssm {M} MMinusD]"
+| "instruction_conv Neg = [AAssm 0, CAssm {A} (Reg M), CAssm {M} (NegR M)]"
+| "instruction_conv Eq = undefined"
+| "instruction_conv Gt = undefined"
+| "instruction_conv Lt = undefined"
+| "instruction_conv And = [AAssm 0, CAssm {A} (Reg M), CAssm {D} (Reg M), AAssm 0, CAssm {A, M} (Decr M), CAssm {M} DAndM]"
+| "instruction_conv Or = [AAssm 0, CAssm {A} (Reg M), CAssm {D} (Reg M), AAssm 0, CAssm {A, M} (Decr M), CAssm {M} DOrM]"
+| "instruction_conv Not = [AAssm 0, CAssm {A} (Reg M), CAssm {D} (NotR M)]"
+
+fun program_convert :: "stack_program \<Rightarrow> assembly_program" where
+  "program_convert [] = []"
+ |"program_convert ((s, \<pi>) # \<Pi>) = (s, concat (map instruction_conv \<pi>)) # program_convert \<Pi>"
+
+primrec stack_to_mem :: "int list \<Rightarrow> (int \<Rightarrow> int) \<Rightarrow> int \<Rightarrow> int" where
+  "stack_to_mem [] \<mu> k = \<mu> k"
+| "stack_to_mem (i # is) \<mu> k = (if k > 0 \<and> nat k = Suc (length is) then i else stack_to_mem is \<mu> k)" 
+
+primrec state_convert :: "stack_state \<Rightarrow> assembly_state set" where
+  "state_convert (\<sigma>, \<pi>) = {((stack_to_mem \<sigma> \<mu>)(0 := int (length \<sigma>)), None, d, concat (map instruction_conv \<pi>)) | d \<mu>. True }"
+
+(* conversion correctness *)
+
+lemma eval_stack_conv [simp]: "eval_stack \<Pi> \<Sigma> = Some \<Sigma>\<^sub>1 \<Longrightarrow> \<Sigma>' \<in> state_convert \<Sigma> \<Longrightarrow> 
+    \<exists>\<Sigma>\<^sub>1'. \<Sigma>\<^sub>1' \<in> state_convert \<Sigma>\<^sub>1 \<and> iterate (eval_assembly (program_convert \<Pi>)) \<Sigma>' \<Sigma>\<^sub>1'"
+  proof (induction \<Pi> \<Sigma> rule: eval_stack.induct)
+  case (1 \<Pi> i1 i2 \<sigma> \<pi>)
+    then obtain d \<mu> where M: "\<Sigma>' = ((stack_to_mem (i1 # i2 # \<sigma>) \<mu>)(0 :=  int (Suc (Suc (length \<sigma>)))), None, d, concat (map instruction_conv (Add # \<pi>)))" by fastforce
+    from 1 have S: "\<Sigma>\<^sub>1 = ((i2 + i1) # \<sigma>, \<pi>)" by simp
+
+    let ?ev = "eval_assembly (program_convert \<Pi>)"
+    let ?\<mu>' = "(stack_to_mem (i1 # i2 # \<sigma>) \<mu>)(0 :=  int (Suc (Suc (length \<sigma>))))"
+
+    have step1: "?ev (?\<mu>', None, d, [AAssm 0, CAssm {A} (Reg M), CAssm {D} (Reg M), AAssm 0, CAssm {A, M} (Decr M), CAssm {M} DPlusM] @ concat (map instruction_conv \<pi>)) = 
+      Some (?\<mu>', Some 0, d, [CAssm {A} (Reg M), CAssm {D} (Reg M), AAssm 0, CAssm {A, M} (Decr M), CAssm {M} DPlusM] @ concat (map instruction_conv \<pi>))" by simp
+    have step2: "?ev (?\<mu>', Some 0, d, [CAssm {A} (Reg M), CAssm {D} (Reg M), AAssm 0, CAssm {A, M} (Decr M), CAssm {M} DPlusM] @ concat (map instruction_conv \<pi>)) = 
+      Some (?\<mu>', Some (?\<mu>' 0), d, [CAssm {D} (Reg M), AAssm 0, CAssm {A, M} (Decr M), CAssm {M} DPlusM] @ concat (map instruction_conv \<pi>))" by simp
+    have step3: "?ev (?\<mu>', Some (?\<mu>' 0), d, [CAssm {D} (Reg M), AAssm 0, CAssm {A, M} (Decr M), CAssm {M} DPlusM] @ concat (map instruction_conv \<pi>)) = 
+      Some (?\<mu>', Some (?\<mu>' 0), ?\<mu>' (?\<mu>' 0), [AAssm 0, CAssm {A, M} (Decr M), CAssm {M} DPlusM] @ concat (map instruction_conv \<pi>))" by simp
+    have step4: "?ev (?\<mu>', Some (?\<mu>' 0), ?\<mu>' (?\<mu>' 0), [AAssm 0, CAssm {A, M} (Decr M), CAssm {M} DPlusM] @ concat (map instruction_conv \<pi>)) = 
+      Some (?\<mu>', Some 0, ?\<mu>' (?\<mu>' 0), [CAssm {A, M} (Decr M), CAssm {M} DPlusM] @ concat (map instruction_conv \<pi>))" by simp
+    have step5: "?ev (?\<mu>', Some 0, ?\<mu>' (?\<mu>' 0), [CAssm {A, M} (Decr M), CAssm {M} DPlusM] @ concat (map instruction_conv \<pi>)) = 
+      Some (?\<mu>'(0 := ?\<mu>' 0 - 1), Some (?\<mu>' 0 - 1), ?\<mu>' (?\<mu>' 0), [CAssm {M} DPlusM] @ concat (map instruction_conv \<pi>))" by simp
+    have step6: "?ev (?\<mu>'(0 := ?\<mu>' 0 - 1), Some (?\<mu>' 0 - 1), ?\<mu>' (?\<mu>' 0), [CAssm {M} DPlusM] @ concat (map instruction_conv \<pi>)) = 
+      Some (?\<mu>'(0 := ?\<mu>' 0 - 1, ?\<mu>' 0 - 1 := ?\<mu>' (?\<mu>' 0) + ?\<mu>' (?\<mu>' 0 - 1)), Some (?\<mu>' 0 - 1), ?\<mu>' (?\<mu>' 0), concat (map instruction_conv \<pi>))" by simp
 
 
 
+    have "\<Sigma>\<^sub>1' \<in> state_convert ((i2 + i1) # \<sigma>, \<pi>) \<and> iterate ?ev (?\<mu>', None, d, [AAssm 0, CAssm {A} (Reg M), CAssm {D} (Reg M), AAssm 0, CAssm {A, M} (Decr M), CAssm {M} DPlusM] @ concat (map instruction_conv \<pi>)) \<Sigma>\<^sub>1'" by simp
+    hence "\<Sigma>\<^sub>1' \<in> state_convert ((i2 + i1) # \<sigma>, \<pi>) \<and> iterate ?ev (?\<mu>', None, d, concat (map instruction_conv (Add # \<pi>))) \<Sigma>\<^sub>1'" by simp
+    with S M show ?case by blast
+  next case 2
+    thus ?case by simp
+  next case 3
+    thus ?case by simp
+  next case 4
+    thus ?case by simp
+  next case 5
+    thus ?case by simp
+  next case 6
+    thus ?case by simp
+  next case 7
+    thus ?case by simp
+  next case 8
+    thus ?case by simp
+  next case 9
+    thus ?case by simp
 
+  (* autogenerated cases where "eval_stack \<Pi> \<Sigma> = None" *)
+  next case "10_1" thus ?case by simp
+  next case "10_2" thus ?case by simp
+  next case "10_3" thus ?case by simp
+  next case "10_4" thus ?case by simp
+  next case "10_5" thus ?case by simp
+  next case "10_6" thus ?case by simp
+  next case "10_7" thus ?case by simp
+  next case "10_8" thus ?case by simp
+  next case "10_9" thus ?case by simp
+  next case "10_10" thus ?case by simp
+  next case "10_11" thus ?case by simp
+  next case "10_12" thus ?case by simp
+  next case "10_13" thus ?case by simp
+  next case "10_14" thus ?case by simp
+  next case "10_15" thus ?case by simp
+  next case "10_16" thus ?case by simp
+  next case "10_17" thus ?case by simp
+  next case "10_18" thus ?case by simp
+  next case "10_19" thus ?case by simp
+  next case "10_20" thus ?case by simp
+  next case "10_21" thus ?case by simp
+  next case "10_22" thus ?case by simp
+  next case "10_23" thus ?case by simp
+  next case "10_24" thus ?case by simp
+  qed
+
+theorem stack_to_assembly_correct [simp]: "iterate (eval_stack \<Pi>) \<Sigma> \<Sigma>\<^sub>1 \<Longrightarrow> \<Sigma>' \<in> state_convert \<Sigma> \<Longrightarrow> 
+    \<exists>\<Sigma>\<^sub>1'. \<Sigma>\<^sub>1' \<in> state_convert \<Sigma>\<^sub>1 \<and> iterate (eval_assembly (program_convert \<Pi>)) \<Sigma>' \<Sigma>\<^sub>1'"
+  proof (induction "eval_stack \<Pi>" \<Sigma> \<Sigma>\<^sub>1 arbitrary: \<Sigma>' rule: iterate.induct)
+  case iter_refl
+    thus ?case by fastforce
+  next case (iter_step \<Sigma> \<Sigma>\<^sub>1 \<Sigma>\<^sub>2)
+    then obtain \<Sigma>\<^sub>1' where S: "\<Sigma>\<^sub>1' \<in> state_convert \<Sigma>\<^sub>1 \<and> 
+      iterate (eval_assembly (program_convert \<Pi>)) \<Sigma>' \<Sigma>\<^sub>1'" by blast
+    with iter_step eval_stack_conv obtain \<Sigma>\<^sub>2' where
+      "\<Sigma>\<^sub>2' \<in> state_convert \<Sigma>\<^sub>2 \<and> iterate (eval_assembly (program_convert \<Pi>)) \<Sigma>\<^sub>1' \<Sigma>\<^sub>2'" by blast
+    with S have "\<Sigma>\<^sub>2' \<in> state_convert \<Sigma>\<^sub>2 \<and> iterate (eval_assembly (program_convert \<Pi>)) \<Sigma>' \<Sigma>\<^sub>2'" 
+      by fastforce
+    thus ?case by blast
+  qed
 
 end
